refactoring dependence analysis to allow incremental analysis of declarations for interactive mode

src/parser/FStarC.Parser.Dep.fst
@@ -608,6 +608,600 @@ let prelude : list (open_kind & lid) = [
 let peek_past_interfaces () =
   if Options.Ext.enabled "dep_minimal" then false else not (Options.ide ())
 
+let collect_module_or_decls (filename:string) (m:either modul (list decl)) : parsing_data =
+  //parse the file and traverse the AST to collect parsing data
+  let num_of_toplevelmods = mk_ref 0 in
+  let pd : ref parsing_data = mk_ref empty_parsing_data in
+
+  let add_to_parsing_data elt =
+    if not (List.existsML (fun e -> parsing_data_elt_eq e elt) (!pd).elts)
+    then pd := { !pd with elts = elt::(!pd).elts }
+  in
+
+  let set_no_prelude b =
+    pd := { !pd with no_prelude = b }
+  in
+
+  let rec go = function
+    | Inl (Module {no_prelude; mname; decls})
+    | Inl (Interface {no_prelude; mname; decls}) ->
+        set_no_prelude no_prelude;
+        // check_module_declaration_against_filename mname filename;
+        add_to_parsing_data (P_begin_module mname);
+        collect_decls decls
+    | Inr decls ->
+        set_no_prelude true;
+        collect_decls decls
+
+  and collect_decls decls =
+    List.iter (fun x -> collect_decl x.d;
+                        List.iter collect_term x.attrs;
+                        match x.d with
+                        | _ when List.contains Inline_for_extraction x.quals ->
+                            add_to_parsing_data P_inline_for_extraction
+                        | _ -> ()
+                        ) decls
+
+  and collect_decl d =
+    match d with
+    | Include (lid, _)
+    | Open (lid, _) ->
+        add_to_parsing_data (P_open (false, lid))
+    | Friend lid ->
+        add_to_parsing_data (P_dep (true, (lowercase_join_longident lid true |> Ident.lid_of_str)))
+    | ModuleAbbrev (ident, lid) ->
+        add_to_parsing_data (P_alias (ident, lid))
+    | TopLevelLet (_, patterms) ->
+        List.iter (fun (pat, t) -> collect_pattern pat; collect_term t) patterms
+    | Splice (_, _, t)
+    | Assume (_, t)
+    | SubEffect { lift_op = NonReifiableLift t }
+    | SubEffect { lift_op = LiftForFree t }
+    | Val (_, t) ->
+        collect_term t
+    | SubEffect { lift_op = ReifiableLift (t0, t1) } ->
+        collect_term t0;
+        collect_term t1
+    | Tycon (_, tc, ts) ->
+        begin
+        if tc then
+            add_to_parsing_data (P_lid Const.tcclass_lid);
+        List.iter collect_tycon ts
+        end
+    | Exception (_, t) ->
+        Option.iter collect_term t
+    | NewEffect ed
+    | LayeredEffect ed ->
+          collect_effect_decl ed
+
+    | Polymonadic_bind (_, _, _, t)
+    | Polymonadic_subcomp (_, _, t) -> collect_term t  //collect deps from the effect lids?
+
+    | DeclToBeDesugared tbs ->
+        tbs.dep_scan 
+        { scan_term = collect_term;
+          scan_binder = collect_binder;
+          scan_pattern = collect_pattern;
+          add_lident = (fun lid -> add_to_parsing_data (P_lid lid));
+          add_open = (fun lid -> add_to_parsing_data (P_open (true, lid)))
+        }
+        tbs.blob
+
+    | UseLangDecls _
+    | Pragma _
+    | DeclSyntaxExtension _
+    | Unparseable ->
+        ()
+    | TopLevelModule lid ->
+        incr num_of_toplevelmods;
+        if (!num_of_toplevelmods > 1) then
+          raise_error lid Errors.Fatal_OneModulePerFile
+            (Format.fmt1 "Automatic dependency analysis demands one module per file (module %s not supported)" (string_of_lid lid true)) 
+  and collect_tycon = function
+    | TyconAbstract (_, binders, k) ->
+        collect_binders binders;
+        Option.iter collect_term k
+    | TyconAbbrev (_, binders, k, t) ->
+        collect_binders binders;
+        Option.iter collect_term k;
+        collect_term t
+    | TyconRecord (_, binders, k, _, identterms) ->
+        collect_binders binders;
+        Option.iter collect_term k;
+        collect_tycon_record identterms
+    | TyconVariant (_, binders, k, identterms) ->
+        collect_binders binders;
+        Option.iter collect_term k;
+        List.iter ( function
+                  | VpOfNotation t | VpArbitrary t -> collect_term t
+                  | VpRecord (record, t) -> collect_tycon_record record;
+                                            Option.iter collect_term t
+                  ) (List.filter_map Mktuple3?._2 identterms)
+
+  and collect_tycon_record r = 
+    List.iter (fun (_, aq, attrs, t) ->
+            collect_aqual aq;
+            attrs |> List.iter collect_term;
+            collect_term t) r
+
+  and collect_effect_decl = function
+    | DefineEffect (_, binders, t, decls) ->
+        collect_binders binders;
+        collect_term t;
+        collect_decls decls
+    | RedefineEffect (_, binders, t) ->
+        collect_binders binders;
+        collect_term t
+
+  and collect_binders binders =
+    List.iter collect_binder binders
+
+  and collect_binder b =
+    collect_aqual b.aqual;
+    b.battributes |> List.iter collect_term;
+    match b with
+    | { b = Annotated (_, t) }
+    | { b = NoName t } -> collect_term t
+    | _ -> ()
+
+  and collect_aqual = function
+    | Some (Meta t) -> collect_term t
+    | Some TypeClassArg -> add_to_parsing_data (P_lid Const.tcresolve_lid)
+    | _ -> ()
+
+  and collect_term t =
+    collect_term' t.tm
+
+  and collect_constant = function
+    | Const_int (_, Some (Unsigned, Sizet)) ->
+        add_to_parsing_data (P_dep (false, ("fstar.sizeT" |> Ident.lid_of_str)))
+    | Const_int (_, Some (signedness, width)) ->
+        let u = match signedness with | Unsigned -> "u" | Signed -> "" in
+        let w = match width with | Int8 -> "8" | Int16 -> "16" | Int32 -> "32" | Int64 -> "64" in
+        add_to_parsing_data (P_dep (false, (Format.fmt2 "fstar.%sint%s" u w |> Ident.lid_of_str)))
+    | Const_char _ ->
+        add_to_parsing_data (P_dep (false, ("fstar.char" |> Ident.lid_of_str)))
+    | Const_range_of
+    | Const_set_range_of ->
+        add_to_parsing_data (P_dep (false, ("fstar.range" |> Ident.lid_of_str)))
+    | Const_real _ ->
+        (* FStar.Real has a real literal it, don't add a circular dep. *)
+        let mm = maybe_module_name_of_file filename in
+        if mm <> Some "FStar.Real" then
+          add_to_parsing_data (P_dep (false, ("fstar.real" |> Ident.lid_of_str)))
+    | _ ->
+        ()
+
+  and collect_term' = function
+    | Wild ->
+        ()
+    | Const c ->
+        collect_constant c
+    | Op (_, ts) ->
+        List.iter collect_term ts
+    | AST.Uvar _ ->
+        ()
+    | Var lid
+    | AST.Projector (lid, _)
+    | AST.Discrim lid
+    | Name lid ->
+        add_to_parsing_data (P_lid lid)
+    | Construct (lid, termimps) ->
+        add_to_parsing_data (P_lid lid);
+        List.iter (fun (t, _) -> collect_term t) termimps
+    | Function (branches, _) ->
+      collect_branches branches
+    | Abs (pats, t) ->
+        collect_patterns pats;
+        collect_term t
+    | App (t1, t2, _) ->
+        collect_term t1;
+        collect_term t2
+    | Let (_, patterms, t) ->
+        List.iter (fun (attrs_opt, (pat, t)) ->
+            ignore (Option.map (List.iter collect_term) attrs_opt);
+            collect_pattern pat;
+            collect_term t)
+            patterms;
+        collect_term t
+    | LetOperator (lets, body) ->
+        List.iter (fun (ident, pat, def) ->
+            collect_pattern pat;
+            collect_term def
+        ) lets;
+        collect_term body
+    | LetOpen (lid, t) ->
+        add_to_parsing_data (P_open (true, lid));
+        collect_term t
+    | LetOpenRecord (r, rty, e) ->
+        collect_term r;
+        collect_term rty;
+        collect_term e
+    | Bind(_, t1, t2)
+    | Seq (t1, t2) ->
+        collect_term t1;
+        collect_term t2
+    | If (t1, _, ret_opt, t2, t3) ->
+        collect_term t1;
+        (match ret_opt with
+          | None -> ()
+          | Some (_, ret, _) ->
+            collect_term ret);
+        collect_term t2;
+        collect_term t3
+    | Match (t, _, ret_opt, bs) ->
+        collect_term t;
+        (match ret_opt with
+          | None -> ()
+          | Some (_, ret, _) ->
+            collect_term ret);
+        collect_branches bs
+    | TryWith (t, bs) ->
+        collect_term t;
+        collect_branches bs
+    | Ascribed (t1, t2, None, _) ->
+        collect_term t1;
+        collect_term t2
+    | Ascribed (t1, t2, Some tac, _) ->
+        collect_term t1;
+        collect_term t2;
+        collect_term tac
+    | Record (t, idterms) ->
+        Option.iter collect_term t;
+        List.iter
+          (fun (fn, t) ->
+            collect_fieldname fn;
+            collect_term t)
+          idterms
+    | Project (t, f) ->
+        collect_term t;
+        collect_fieldname f
+    | Product (binders, t) ->
+      collect_binders binders;
+      collect_term t
+    | Sum (binders, t) ->
+        List.iter (function
+          | Inl b -> collect_binder b
+          | Inr t -> collect_term t)
+          binders;
+        collect_term t
+    | QForall (binders, (_, ts), t)
+    | QExists (binders, (_, ts), t)
+    | QuantOp (_, binders, (_, ts), t) ->
+        collect_binders binders;
+        List.iter (List.iter collect_term) ts;
+        collect_term t
+    | Refine (binder, t) ->
+        collect_binder binder;
+        collect_term t
+    | NamedTyp (_, t) ->
+        collect_term t
+    | Paren t ->
+        collect_term t
+    | Requires t
+    | Ensures t
+    | Labeled (t, _, _) ->
+        collect_term t
+    | LexList l -> List.iter collect_term l
+    | WFOrder (t1, t2) ->
+      add_to_parsing_data (P_dep (false, (Ident.lid_of_str "FStar.WellFounded")));
+      begin
+        collect_term t1; collect_term t2
+      end
+    | Decreases t -> collect_term t
+    | Quote (t, _)
+    | Antiquote t
+    | VQuote t ->
+        collect_term t
+    | Attributes cattributes  ->
+        List.iter collect_term cattributes
+    | CalcProof (rel, init, steps) ->
+        add_to_parsing_data (P_dep (false, (Ident.lid_of_str "FStar.Calc")));
+        begin
+        collect_term rel;
+        collect_term init;
+        List.iter (function CalcStep (rel, just, next) ->
+            collect_term rel;
+            collect_term just;
+            collect_term next) steps
+        end
+
+    | IntroForall (bs, p, e) ->
+      add_to_parsing_data (P_dep (false, (Ident.lid_of_str "FStar.Classical.Sugar")));
+      collect_binders bs;
+      collect_term p;
+      collect_term e
+
+    | IntroExists(bs, t, vs, e) ->
+      add_to_parsing_data (P_dep (false, (Ident.lid_of_str "FStar.Classical.Sugar")));
+      collect_binders bs;
+      collect_term t;
+      List.iter collect_term vs;
+      collect_term e
+
+    | IntroImplies(p, q, x, e) ->
+      add_to_parsing_data (P_dep (false, (Ident.lid_of_str "FStar.Classical.Sugar")));
+      collect_term p;
+      collect_term q;
+      collect_binder x;
+      collect_term e
+
+    | IntroOr(b, p, q, r) ->
+      add_to_parsing_data (P_dep (false, (Ident.lid_of_str "FStar.Classical.Sugar")));
+      collect_term p;
+      collect_term q;
+      collect_term r
+
+    | IntroAnd(p, q, r, e) ->
+      add_to_parsing_data (P_dep (false, (Ident.lid_of_str "FStar.Classical.Sugar")));
+      collect_term p;
+      collect_term q;
+      collect_term r;
+      collect_term e
+
+    | ElimForall(bs, p, vs) ->
+        add_to_parsing_data (P_dep (false, (Ident.lid_of_str "FStar.Classical.Sugar")));
+        collect_binders bs;
+        collect_term p;
+        List.iter collect_term vs
+
+    | ElimExists(bs, p, q, b, e) ->
+        add_to_parsing_data (P_dep (false, (Ident.lid_of_str "FStar.Classical.Sugar")));
+        collect_binders bs;
+        collect_term p;
+        collect_term q;
+        collect_binder b;
+        collect_term e
+
+    | ElimImplies(p, q, e) ->
+      add_to_parsing_data (P_dep (false, (Ident.lid_of_str "FStar.Classical.Sugar")));
+      collect_term p;
+      collect_term q;
+      collect_term e
+
+    | ElimAnd(p, q, r, x, y, e) ->
+      add_to_parsing_data (P_dep (false, (Ident.lid_of_str "FStar.Classical.Sugar")));
+      collect_term p;
+      collect_term q;
+      collect_term r;
+      collect_binder x;
+      collect_binder y;
+      collect_term e
+
+    | ElimOr(p, q, r, x, e, y, e') ->
+      add_to_parsing_data (P_dep (false, (Ident.lid_of_str "FStar.Classical.Sugar")));
+      collect_term p;
+      collect_term q;
+      collect_term r;
+      collect_binder x;
+      collect_binder y;
+      collect_term e;
+      collect_term e'
+
+    | ListLiteral ts ->
+      List.iter collect_term ts
+
+    | SeqLiteral ts ->
+      add_to_parsing_data (P_dep (false, (Ident.lid_of_str "FStar.Seq.Base")));
+      List.iter collect_term ts
+    
+  and collect_patterns ps =
+    List.iter collect_pattern ps
+
+  and collect_pattern p =
+    collect_pattern' p.pat
+
+  and collect_pattern' = function
+    | PatVar (_, aqual, attrs)
+    | PatWild (aqual, attrs) ->
+        collect_aqual aqual;
+        attrs |> List.iter collect_term
+
+    | PatRest
+    | PatOp _
+    | PatConst _ ->
+        ()
+    | PatVQuote t ->
+        collect_term t
+    | PatApp (p, ps) ->
+        collect_pattern p;
+        collect_patterns ps
+    | PatName lid ->
+        add_to_parsing_data (P_lid lid)
+    | PatList ps
+    | PatOr ps
+    | PatTuple (ps, _) ->
+        collect_patterns ps
+    | PatRecord lidpats ->
+        List.iter (fun (_, p) -> collect_pattern p) lidpats
+    | PatAscribed (p, (t, None)) ->
+        collect_pattern p;
+        collect_term t
+    | PatAscribed (p, (t, Some tac)) ->
+        collect_pattern p;
+        collect_term t;
+        collect_term tac
+
+
+  and collect_branches bs =
+    List.iter collect_branch bs
+
+  and collect_branch (pat, t1, t2) =
+    collect_pattern pat;
+    Option.iter collect_term t1;
+    collect_term t2
+
+  and collect_fieldname fn =
+      if nsstr fn <> ""
+      then add_to_parsing_data (P_dep (false, lid_of_ids (ns_of_lid fn)))
+  in
+  go m;
+  !pd
+
+
+(*
+  * Construct dependences from the parsing data
+  * This is common function for when the parsing data is read from the checked files
+  *   or constructed after AST traversal of the module
+  *)
+let deps_from_parsing_data (pd:parsing_data) (original_map:files_for_module_name) (filename:string)
+: list dependence & //direct dependences
+  bool &            //has inline for extraction
+  list dependence   //additional roots
+= 
+  let deps     : ref (list dependence) = mk_ref [] in
+  let has_inline_for_extraction = mk_ref false in
+
+  let mname = lowercase_module_name filename in
+  let mo_roots =
+    if is_interface filename
+    && has_implementation original_map mname
+    && peek_past_interfaces()
+    then [ UseImplementation mname ]
+    else []
+  in
+
+  let auto_open =
+    if pd.no_prelude
+    then []
+    else
+      (prelude |> List.map (fun (k, l) -> P_open (false, l)))
+      @
+      (match namespace_of_module mname with
+        | None -> []
+        | Some ns -> [ P_implicit_open_module_or_namespace (Open_namespace, ns) ])
+  in
+
+  let working_map = SMap.copy original_map in
+
+  let set_interface_inlining () =
+    if is_interface filename
+    then has_inline_for_extraction := true
+  in
+
+  let add_dep deps d =
+    if not (List.existsML (dep_subsumed_by d) !deps) then
+      deps := d :: !deps
+  in
+
+  let dep_edge module_name is_friend =
+    if is_friend then FriendImplementation module_name
+    else PreferInterface module_name
+  in
+
+  let add_dependence_edge original_or_working_map lid is_friend =
+    let key = lowercase_join_longident lid true in
+    match resolve_module_name original_or_working_map key with
+    | Some module_name ->
+      add_dep deps (dep_edge module_name is_friend);
+      true
+    | _ ->
+      false
+  in
+
+  let record_open_module let_open lid =
+    //use the original_map here
+    //since the working_map will resolve lid while accounting
+    //for already opened namespaces
+    //if let_open, then this is the form `UInt64.( ... )`
+    //             where UInt64 can resolve to FStar.UInt64
+    //           So, use the working map, accounting for opened namespaces
+    //Otherwise, this is the form `open UInt64`,
+    //           where UInt64 must resolve to either
+    //           a module or a namespace for F# compatibility
+    //           So, use the original map, disregarding opened namespaces
+    if (let_open     && add_dependence_edge working_map lid false)
+    || (not let_open && add_dependence_edge original_map lid false)
+    then true
+    else begin
+      if let_open then
+        log_issue lid Errors.Warning_ModuleOrFileNotFoundWarning
+          (Format.fmt1 "Module not found: %s" (string_of_lid lid true));
+      false
+    end
+  in
+
+  let record_open_namespace lid (implicit_open:bool) =
+    let key = lowercase_join_longident lid true in
+    let r = enter_namespace original_map working_map key implicit_open in
+    if not r && not implicit_open then  //suppress the warning for implicit opens
+      log_issue lid Errors.Warning_ModuleOrFileNotFoundWarning
+        (Format.fmt1 "No modules in namespace %s and no file with that name either" (string_of_lid lid true))
+  in
+
+  let record_open let_open lid =
+    if record_open_module let_open lid
+    then ()
+    else if not let_open //syntactically, this cannot be a namespace if let_open is true; so don't retry
+    then record_open_namespace lid false
+  in
+
+  let record_implicit_open_module_or_namespace (lid, kind) =
+    match kind with
+    | Open_namespace -> record_open_namespace lid true
+    | Open_module -> let _ = record_open_module false lid in ()
+  in
+
+  let record_module_alias ident lid =
+    let key = String.lowercase (string_of_id ident) in
+    let alias = lowercase_join_longident lid true in
+    // Only fully qualified module aliases are allowed.
+    match SMap.try_find original_map alias with
+    | Some deps_of_aliased_module ->
+      SMap.add working_map key deps_of_aliased_module;
+      add_dep deps (dep_edge (lowercase_join_longident lid true) false);
+      true
+    | None ->
+      log_issue lid Errors.Warning_ModuleOrFileNotFoundWarning
+        (Format.fmt1 "module not found in search path: %s" alias);
+      false
+  in
+
+  let add_dep_on_module (module_name : lid) (is_friend : bool) =
+    if add_dependence_edge working_map module_name is_friend
+    then ()
+    else if !dbg then
+      log_issue module_name Errors.Warning_UnboundModuleReference
+        (Format.fmt1 "Unbound module reference %s" (show module_name))
+  in
+
+  let record_lid lid =
+    (* Thanks to the new `?.` and `.(` syntaxes, `lid` is no longer a
+      module name itself, so only its namespace part is to be
+      recorded as a module dependency.  *)
+    match ns_of_lid lid with
+    | [] -> ()
+    | ns ->
+      let module_name = Ident.lid_of_ids ns in
+      add_dep_on_module module_name false
+  in
+
+  let begin_module lid =
+    if List.length (ns_of_lid lid) > 0 then
+    ignore (enter_namespace original_map working_map (namespace_of_lid lid))
+  in
+
+  (*
+  * Iterate over the parsing data elements
+  *)
+  begin
+    (auto_open @ pd.elts) |> List.iter (fun elt ->
+      match elt with
+      | P_begin_module lid -> begin_module lid
+      | P_open (b, lid) -> record_open b lid
+      | P_implicit_open_module_or_namespace (k, lid) -> record_implicit_open_module_or_namespace (lid, k)
+      | P_dep (b, lid) -> add_dep_on_module lid b
+      | P_alias (id, lid) -> ignore (record_module_alias id lid)
+      | P_lid lid -> record_lid lid
+      | P_inline_for_extraction -> set_interface_inlining ())
+  end;
+  (*
+  * And then return the dependences
+  *)
+  !deps,
+  !has_inline_for_extraction,
+  mo_roots
+
 (*
  * Get parsing data for a file
  * First see if the data in the checked file is good (using the provided callback)
@@ -629,608 +1223,21 @@ let collect_one
                       //removing it from the cache (#1657)
                       //this always returns a single element, remove the list?
 =
-  (*
-   * Construct dependences from the parsing data
-   * This is common function for when the parsing data is read from the checked files
-   *   or constructed after AST traversal of the module
-   *)
-  let from_parsing_data (pd:parsing_data) (original_map:files_for_module_name) (filename:string)
-    : list dependence &
-      bool &
-      list dependence
-    =  let deps     : ref (list dependence) = mk_ref [] in
-       let has_inline_for_extraction = mk_ref false in
-
-       let mname = lowercase_module_name filename in
-       let mo_roots =
-         if is_interface filename
-         && has_implementation original_map mname
-         && peek_past_interfaces()
-         then [ UseImplementation mname ]
-         else []
-       in
-
-       let auto_open =
-         if pd.no_prelude
-         then []
-         else
-           (prelude |> List.map (fun (k, l) -> P_open (false, l)))
-           @
-           (match namespace_of_module mname with
-             | None -> []
-             | Some ns -> [ P_implicit_open_module_or_namespace (Open_namespace, ns) ])
-       in
-
-       let working_map = SMap.copy original_map in
-
-       let set_interface_inlining () =
-         if is_interface filename
-         then has_inline_for_extraction := true
-       in
-
-       let add_dep deps d =
-         if not (List.existsML (dep_subsumed_by d) !deps) then
-           deps := d :: !deps
-       in
-
-       let dep_edge module_name is_friend =
-         if is_friend then FriendImplementation module_name
-         else PreferInterface module_name
-       in
-
-       let add_dependence_edge original_or_working_map lid is_friend =
-         let key = lowercase_join_longident lid true in
-         match resolve_module_name original_or_working_map key with
-         | Some module_name ->
-           add_dep deps (dep_edge module_name is_friend);
-           true
-         | _ ->
-           false
-       in
-
-       let record_open_module let_open lid =
-         //use the original_map here
-         //since the working_map will resolve lid while accounting
-         //for already opened namespaces
-         //if let_open, then this is the form `UInt64.( ... )`
-         //             where UInt64 can resolve to FStar.UInt64
-         //           So, use the working map, accounting for opened namespaces
-         //Otherwise, this is the form `open UInt64`,
-         //           where UInt64 must resolve to either
-         //           a module or a namespace for F# compatibility
-         //           So, use the original map, disregarding opened namespaces
-         if (let_open     && add_dependence_edge working_map lid false)
-         || (not let_open && add_dependence_edge original_map lid false)
-         then true
-         else begin
-           if let_open then
-             log_issue lid Errors.Warning_ModuleOrFileNotFoundWarning
-               (Format.fmt1 "Module not found: %s" (string_of_lid lid true));
-           false
-         end
-       in
-
-       let record_open_namespace lid (implicit_open:bool) =
-         let key = lowercase_join_longident lid true in
-         let r = enter_namespace original_map working_map key implicit_open in
-         if not r && not implicit_open then  //suppress the warning for implicit opens
-           log_issue lid Errors.Warning_ModuleOrFileNotFoundWarning
-             (Format.fmt1 "No modules in namespace %s and no file with that name either" (string_of_lid lid true))
-       in
-
-       let record_open let_open lid =
-         if record_open_module let_open lid
-         then ()
-         else if not let_open //syntactically, this cannot be a namespace if let_open is true; so don't retry
-         then record_open_namespace lid false
-       in
-
-       let record_implicit_open_module_or_namespace (lid, kind) =
-         match kind with
-         | Open_namespace -> record_open_namespace lid true
-         | Open_module -> let _ = record_open_module false lid in ()
-       in
-
-       let record_module_alias ident lid =
-         let key = String.lowercase (string_of_id ident) in
-         let alias = lowercase_join_longident lid true in
-         // Only fully qualified module aliases are allowed.
-         match SMap.try_find original_map alias with
-         | Some deps_of_aliased_module ->
-           SMap.add working_map key deps_of_aliased_module;
-           add_dep deps (dep_edge (lowercase_join_longident lid true) false);
-           true
-         | None ->
-           log_issue lid Errors.Warning_ModuleOrFileNotFoundWarning
-             (Format.fmt1 "module not found in search path: %s" alias);
-           false
-       in
-
-       let add_dep_on_module (module_name : lid) (is_friend : bool) =
-         if add_dependence_edge working_map module_name is_friend
-         then ()
-         else if !dbg then
-           log_issue module_name Errors.Warning_UnboundModuleReference
-             (Format.fmt1 "Unbound module reference %s" (show module_name))
-       in
-
-       let record_lid lid =
-         (* Thanks to the new `?.` and `.(` syntaxes, `lid` is no longer a
-            module name itself, so only its namespace part is to be
-            recorded as a module dependency.  *)
-         match ns_of_lid lid with
-         | [] -> ()
-         | ns ->
-           let module_name = Ident.lid_of_ids ns in
-           add_dep_on_module module_name false
-       in
-
-       let begin_module lid =
-         if List.length (ns_of_lid lid) > 0 then
-         ignore (enter_namespace original_map working_map (namespace_of_lid lid))
-       in
-
-       (*
-        * Iterate over the parsing data elements
-        *)
-       begin
-         (auto_open @ pd.elts) |> List.iter (fun elt ->
-           match elt with
-           | P_begin_module lid -> begin_module lid
-           | P_open (b, lid) -> record_open b lid
-           | P_implicit_open_module_or_namespace (k, lid) -> record_implicit_open_module_or_namespace (lid, k)
-           | P_dep (b, lid) -> add_dep_on_module lid b
-           | P_alias (id, lid) -> ignore (record_module_alias id lid)
-           | P_lid lid -> record_lid lid
-           | P_inline_for_extraction -> set_interface_inlining ())
-       end;
-       (*
-        * And then return the dependences
-        *)
-       !deps,
-       !has_inline_for_extraction,
-       mo_roots
-  in
-
   let data_from_cache = filename |> get_parsing_data_from_cache in
-
   if data_from_cache |> Some? then begin  //we found the parsing data in the checked file
-    let deps, has_inline_for_extraction, mo_roots = from_parsing_data (data_from_cache |> Option.must) original_map filename in
+    let deps, has_inline_for_extraction, mo_roots =
+      deps_from_parsing_data (data_from_cache |> Option.must) original_map filename
+    in
     if !dbg then
       Format.print2 "Reading the parsing data for %s from its checked file .. found %s\n" filename (show deps);
     data_from_cache |> Option.must,
     deps, has_inline_for_extraction, mo_roots
   end
   else begin
-      //parse the file and traverse the AST to collect parsing data
-      let num_of_toplevelmods = mk_ref 0 in
-      let pd : ref parsing_data = mk_ref empty_parsing_data in
-
-      let add_to_parsing_data elt =
-        if not (List.existsML (fun e -> parsing_data_elt_eq e elt) (!pd).elts)
-        then pd := { !pd with elts = elt::(!pd).elts }
-      in
-
-      let set_no_prelude b =
-        pd := { !pd with no_prelude = b }
-      in
-
-      let rec collect_module = function
-        | Module {no_prelude; mname; decls}
-        | Interface {no_prelude; mname; decls} ->
-            set_no_prelude no_prelude;
-            check_module_declaration_against_filename mname filename;
-            add_to_parsing_data (P_begin_module mname);
-            collect_decls decls
-
-      and collect_decls decls =
-        List.iter (fun x -> collect_decl x.d;
-                            List.iter collect_term x.attrs;
-                            match x.d with
-                            | _ when List.contains Inline_for_extraction x.quals ->
-                                add_to_parsing_data P_inline_for_extraction
-                            | _ -> ()
-                            ) decls
-
-      and collect_decl d =
-        match d with
-        | Include (lid, _)
-        | Open (lid, _) ->
-            add_to_parsing_data (P_open (false, lid))
-        | Friend lid ->
-            add_to_parsing_data (P_dep (true, (lowercase_join_longident lid true |> Ident.lid_of_str)))
-        | ModuleAbbrev (ident, lid) ->
-            add_to_parsing_data (P_alias (ident, lid))
-        | TopLevelLet (_, patterms) ->
-            List.iter (fun (pat, t) -> collect_pattern pat; collect_term t) patterms
-        | Splice (_, _, t)
-        | Assume (_, t)
-        | SubEffect { lift_op = NonReifiableLift t }
-        | SubEffect { lift_op = LiftForFree t }
-        | Val (_, t) ->
-            collect_term t
-        | SubEffect { lift_op = ReifiableLift (t0, t1) } ->
-            collect_term t0;
-            collect_term t1
-        | Tycon (_, tc, ts) ->
-            begin
-            if tc then
-                add_to_parsing_data (P_lid Const.tcclass_lid);
-            List.iter collect_tycon ts
-            end
-        | Exception (_, t) ->
-            Option.iter collect_term t
-        | NewEffect ed
-        | LayeredEffect ed ->
-             collect_effect_decl ed
-
-        | Polymonadic_bind (_, _, _, t)
-        | Polymonadic_subcomp (_, _, t) -> collect_term t  //collect deps from the effect lids?
-
-        | DeclToBeDesugared tbs ->
-            tbs.dep_scan 
-            { scan_term = collect_term;
-              scan_binder = collect_binder;
-              scan_pattern = collect_pattern;
-              add_lident = (fun lid -> add_to_parsing_data (P_lid lid));
-              add_open = (fun lid -> add_to_parsing_data (P_open (true, lid)))
-            }
-            tbs.blob
-
-        | UseLangDecls _
-        | Pragma _
-        | DeclSyntaxExtension _
-        | Unparseable ->
-            ()
-        | TopLevelModule lid ->
-            incr num_of_toplevelmods;
-            if (!num_of_toplevelmods > 1) then
-              raise_error lid Errors.Fatal_OneModulePerFile
-                (Format.fmt1 "Automatic dependency analysis demands one module per file (module %s not supported)" (string_of_lid lid true)) 
-      and collect_tycon = function
-        | TyconAbstract (_, binders, k) ->
-            collect_binders binders;
-            Option.iter collect_term k
-        | TyconAbbrev (_, binders, k, t) ->
-            collect_binders binders;
-            Option.iter collect_term k;
-            collect_term t
-        | TyconRecord (_, binders, k, _, identterms) ->
-            collect_binders binders;
-            Option.iter collect_term k;
-            collect_tycon_record identterms
-        | TyconVariant (_, binders, k, identterms) ->
-            collect_binders binders;
-            Option.iter collect_term k;
-            List.iter ( function
-                      | VpOfNotation t | VpArbitrary t -> collect_term t
-                      | VpRecord (record, t) -> collect_tycon_record record;
-                                               Option.iter collect_term t
-                      ) (List.filter_map Mktuple3?._2 identterms)
-
-      and collect_tycon_record r = 
-        List.iter (fun (_, aq, attrs, t) ->
-                collect_aqual aq;
-                attrs |> List.iter collect_term;
-                collect_term t) r
-
-      and collect_effect_decl = function
-        | DefineEffect (_, binders, t, decls) ->
-            collect_binders binders;
-            collect_term t;
-            collect_decls decls
-        | RedefineEffect (_, binders, t) ->
-            collect_binders binders;
-            collect_term t
-
-      and collect_binders binders =
-        List.iter collect_binder binders
-
-      and collect_binder b =
-        collect_aqual b.aqual;
-        b.battributes |> List.iter collect_term;
-        match b with
-        | { b = Annotated (_, t) }
-        | { b = NoName t } -> collect_term t
-        | _ -> ()
-
-      and collect_aqual = function
-        | Some (Meta t) -> collect_term t
-        | Some TypeClassArg -> add_to_parsing_data (P_lid Const.tcresolve_lid)
-        | _ -> ()
-
-      and collect_term t =
-        collect_term' t.tm
-
-      and collect_constant = function
-        | Const_int (_, Some (Unsigned, Sizet)) ->
-            add_to_parsing_data (P_dep (false, ("fstar.sizeT" |> Ident.lid_of_str)))
-        | Const_int (_, Some (signedness, width)) ->
-            let u = match signedness with | Unsigned -> "u" | Signed -> "" in
-            let w = match width with | Int8 -> "8" | Int16 -> "16" | Int32 -> "32" | Int64 -> "64" in
-            add_to_parsing_data (P_dep (false, (Format.fmt2 "fstar.%sint%s" u w |> Ident.lid_of_str)))
-        | Const_char _ ->
-            add_to_parsing_data (P_dep (false, ("fstar.char" |> Ident.lid_of_str)))
-        | Const_range_of
-        | Const_set_range_of ->
-            add_to_parsing_data (P_dep (false, ("fstar.range" |> Ident.lid_of_str)))
-        | Const_real _ ->
-            (* FStar.Real has a real literal it, don't add a circular dep. *)
-            let mm = maybe_module_name_of_file filename in
-            if mm <> Some "FStar.Real" then
-              add_to_parsing_data (P_dep (false, ("fstar.real" |> Ident.lid_of_str)))
-        | _ ->
-            ()
-
-      and collect_term' = function
-        | Wild ->
-            ()
-        | Const c ->
-            collect_constant c
-        | Op (_, ts) ->
-            List.iter collect_term ts
-        | AST.Uvar _ ->
-            ()
-        | Var lid
-        | AST.Projector (lid, _)
-        | AST.Discrim lid
-        | Name lid ->
-            add_to_parsing_data (P_lid lid)
-        | Construct (lid, termimps) ->
-            add_to_parsing_data (P_lid lid);
-            List.iter (fun (t, _) -> collect_term t) termimps
-        | Function (branches, _) ->
-          collect_branches branches
-        | Abs (pats, t) ->
-            collect_patterns pats;
-            collect_term t
-        | App (t1, t2, _) ->
-            collect_term t1;
-            collect_term t2
-        | Let (_, patterms, t) ->
-            List.iter (fun (attrs_opt, (pat, t)) ->
-                ignore (Option.map (List.iter collect_term) attrs_opt);
-                collect_pattern pat;
-                collect_term t)
-                patterms;
-            collect_term t
-        | LetOperator (lets, body) ->
-            List.iter (fun (ident, pat, def) ->
-                collect_pattern pat;
-                collect_term def
-            ) lets;
-            collect_term body
-        | LetOpen (lid, t) ->
-            add_to_parsing_data (P_open (true, lid));
-            collect_term t
-        | LetOpenRecord (r, rty, e) ->
-            collect_term r;
-            collect_term rty;
-            collect_term e
-        | Bind(_, t1, t2)
-        | Seq (t1, t2) ->
-            collect_term t1;
-            collect_term t2
-        | If (t1, _, ret_opt, t2, t3) ->
-            collect_term t1;
-            (match ret_opt with
-             | None -> ()
-             | Some (_, ret, _) ->
-               collect_term ret);
-            collect_term t2;
-            collect_term t3
-        | Match (t, _, ret_opt, bs) ->
-            collect_term t;
-            (match ret_opt with
-             | None -> ()
-             | Some (_, ret, _) ->
-               collect_term ret);
-            collect_branches bs
-        | TryWith (t, bs) ->
-            collect_term t;
-            collect_branches bs
-        | Ascribed (t1, t2, None, _) ->
-            collect_term t1;
-            collect_term t2
-        | Ascribed (t1, t2, Some tac, _) ->
-            collect_term t1;
-            collect_term t2;
-            collect_term tac
-        | Record (t, idterms) ->
-            Option.iter collect_term t;
-            List.iter
-              (fun (fn, t) ->
-                collect_fieldname fn;
-                collect_term t)
-              idterms
-        | Project (t, f) ->
-            collect_term t;
-            collect_fieldname f
-        | Product (binders, t) ->
-          collect_binders binders;
-          collect_term t
-        | Sum (binders, t) ->
-            List.iter (function
-              | Inl b -> collect_binder b
-              | Inr t -> collect_term t)
-              binders;
-            collect_term t
-        | QForall (binders, (_, ts), t)
-        | QExists (binders, (_, ts), t)
-        | QuantOp (_, binders, (_, ts), t) ->
-            collect_binders binders;
-            List.iter (List.iter collect_term) ts;
-            collect_term t
-        | Refine (binder, t) ->
-            collect_binder binder;
-            collect_term t
-        | NamedTyp (_, t) ->
-            collect_term t
-        | Paren t ->
-            collect_term t
-        | Requires t
-        | Ensures t
-        | Labeled (t, _, _) ->
-            collect_term t
-        | LexList l -> List.iter collect_term l
-        | WFOrder (t1, t2) ->
-          add_to_parsing_data (P_dep (false, (Ident.lid_of_str "FStar.WellFounded")));
-          begin
-           collect_term t1; collect_term t2
-          end
-        | Decreases t -> collect_term t
-        | Quote (t, _)
-        | Antiquote t
-        | VQuote t ->
-            collect_term t
-        | Attributes cattributes  ->
-            List.iter collect_term cattributes
-        | CalcProof (rel, init, steps) ->
-            add_to_parsing_data (P_dep (false, (Ident.lid_of_str "FStar.Calc")));
-            begin
-            collect_term rel;
-            collect_term init;
-            List.iter (function CalcStep (rel, just, next) ->
-                collect_term rel;
-                collect_term just;
-                collect_term next) steps
-            end
-
-        | IntroForall (bs, p, e) ->
-          add_to_parsing_data (P_dep (false, (Ident.lid_of_str "FStar.Classical.Sugar")));
-          collect_binders bs;
-          collect_term p;
-          collect_term e
-
-        | IntroExists(bs, t, vs, e) ->
-          add_to_parsing_data (P_dep (false, (Ident.lid_of_str "FStar.Classical.Sugar")));
-          collect_binders bs;
-          collect_term t;
-          List.iter collect_term vs;
-          collect_term e
-
-        | IntroImplies(p, q, x, e) ->
-          add_to_parsing_data (P_dep (false, (Ident.lid_of_str "FStar.Classical.Sugar")));
-          collect_term p;
-          collect_term q;
-          collect_binder x;
-          collect_term e
-
-        | IntroOr(b, p, q, r) ->
-          add_to_parsing_data (P_dep (false, (Ident.lid_of_str "FStar.Classical.Sugar")));
-          collect_term p;
-          collect_term q;
-          collect_term r
-
-        | IntroAnd(p, q, r, e) ->
-          add_to_parsing_data (P_dep (false, (Ident.lid_of_str "FStar.Classical.Sugar")));
-          collect_term p;
-          collect_term q;
-          collect_term r;
-          collect_term e
-
-        | ElimForall(bs, p, vs) ->
-           add_to_parsing_data (P_dep (false, (Ident.lid_of_str "FStar.Classical.Sugar")));
-           collect_binders bs;
-           collect_term p;
-           List.iter collect_term vs
-
-        | ElimExists(bs, p, q, b, e) ->
-           add_to_parsing_data (P_dep (false, (Ident.lid_of_str "FStar.Classical.Sugar")));
-           collect_binders bs;
-           collect_term p;
-           collect_term q;
-           collect_binder b;
-           collect_term e
-
-        | ElimImplies(p, q, e) ->
-          add_to_parsing_data (P_dep (false, (Ident.lid_of_str "FStar.Classical.Sugar")));
-          collect_term p;
-          collect_term q;
-          collect_term e
-
-        | ElimAnd(p, q, r, x, y, e) ->
-          add_to_parsing_data (P_dep (false, (Ident.lid_of_str "FStar.Classical.Sugar")));
-          collect_term p;
-          collect_term q;
-          collect_term r;
-          collect_binder x;
-          collect_binder y;
-          collect_term e
-
-        | ElimOr(p, q, r, x, e, y, e') ->
-          add_to_parsing_data (P_dep (false, (Ident.lid_of_str "FStar.Classical.Sugar")));
-          collect_term p;
-          collect_term q;
-          collect_term r;
-          collect_binder x;
-          collect_binder y;
-          collect_term e;
-          collect_term e'
-
-        | ListLiteral ts ->
-          List.iter collect_term ts
-
-        | SeqLiteral ts ->
-          add_to_parsing_data (P_dep (false, (Ident.lid_of_str "FStar.Seq.Base")));
-          List.iter collect_term ts
-        
-      and collect_patterns ps =
-        List.iter collect_pattern ps
-
-      and collect_pattern p =
-        collect_pattern' p.pat
-
-      and collect_pattern' = function
-        | PatVar (_, aqual, attrs)
-        | PatWild (aqual, attrs) ->
-            collect_aqual aqual;
-            attrs |> List.iter collect_term
-
-        | PatRest
-        | PatOp _
-        | PatConst _ ->
-            ()
-        | PatVQuote t ->
-            collect_term t
-        | PatApp (p, ps) ->
-            collect_pattern p;
-            collect_patterns ps
-        | PatName lid ->
-            add_to_parsing_data (P_lid lid)
-        | PatList ps
-        | PatOr ps
-        | PatTuple (ps, _) ->
-            collect_patterns ps
-        | PatRecord lidpats ->
-            List.iter (fun (_, p) -> collect_pattern p) lidpats
-        | PatAscribed (p, (t, None)) ->
-            collect_pattern p;
-            collect_term t
-        | PatAscribed (p, (t, Some tac)) ->
-            collect_pattern p;
-            collect_term t;
-            collect_term tac
-
-
-      and collect_branches bs =
-        List.iter collect_branch bs
-
-      and collect_branch (pat, t1, t2) =
-        collect_pattern pat;
-        Option.iter collect_term t1;
-        collect_term t2
-
-      and collect_fieldname fn =
-          if nsstr fn <> ""
-          then add_to_parsing_data (P_dep (false, lid_of_ids (ns_of_lid fn)))
-
-      in
       let ast, _ = Driver.parse_file filename in
-      collect_module ast;
-      let pd = !pd in
+      let pd = collect_module_or_decls filename (Inl ast) in
       let pd = { pd with elts = List.rev pd.elts } in
-      let deps, has_inline_for_extraction, mo_roots = from_parsing_data pd original_map filename in
+      let deps, has_inline_for_extraction, mo_roots = deps_from_parsing_data pd original_map filename in
       (* Util.print2 "Deps for %s: %s\n" filename (String.concat " " (!deps)); *)
       pd, deps, has_inline_for_extraction, mo_roots
     end
@@ -1450,6 +1457,73 @@ let all_files_in_include_paths () =
       List.map (fun file -> Filepath.join_paths path file) files)
     paths
 
+let build_dep_graph_for_files
+      (files:list string)
+      (file_system_map:_)
+      (dep_graph:_)
+      (parse_results:_)
+      (get_parsing_data_from_cache:string -> option parsing_data)
+: list string //interfaces needing inlining
+= (* The dependency graph; keys are lowercased module names, values = list of
+   * lowercased module names this file depends on. *)
+  let interfaces_needing_inlining = mk_ref [] in
+  let add_interface_for_inlining l =
+    let l = lowercase_module_name l in
+    interfaces_needing_inlining := l :: !interfaces_needing_inlining
+  in
+  (* discover: Do a graph traversal starting from file_name
+   *           filling in dep_graph with the dependences *)
+  let rec discover_one (file_name:file_name) : unit =
+    if deps_try_find dep_graph file_name = None then
+    begin
+      let parsing_data, (deps, mo_roots, needs_interface_inlining) =
+        match SMap.try_find !collect_one_cache file_name with
+        | Some cached -> empty_parsing_data, cached
+        | None ->
+          let parsing_data, deps, needs_interface_inlining, additional_roots =
+            collect_one file_system_map file_name get_parsing_data_from_cache
+          in
+          parsing_data, (deps, additional_roots, needs_interface_inlining)
+      in
+      debug_print (fun _ -> 
+        Format.print3 "collect_one (%s) : deps=%s; mo_roots=%s\n"
+          file_name (show deps) (show mo_roots)
+      );
+      if needs_interface_inlining
+      then add_interface_for_inlining file_name;
+      SMap.add parse_results file_name parsing_data;
+      let deps =
+          let module_name = lowercase_module_name file_name in
+          if is_implementation file_name
+          && has_interface file_system_map module_name
+          then deps @ [UseInterface module_name]
+          else deps
+      in
+      let dep_node : dep_node = {
+        edges = List.unique deps;
+        color = White;
+      } in
+      deps_add_dep dep_graph file_name dep_node;
+      List.iter
+            discover_one
+            (List.map (file_of_dep file_system_map files)
+                      (deps @ mo_roots))
+    end
+  in
+  profile (fun () -> List.iter discover_one files) "FStarC.Parser.Dep.discover"; 
+  !interfaces_needing_inlining
+
+
+let collect_deps_of_decl (deps:deps) (filename:string) (ds:list decl)
+  (get_parsing_data_from_cache:string -> option parsing_data)
+: list file_name
+= let pd = collect_module_or_decls filename (Inr ds) in
+  let direct_deps, _has_inline_for_extraction, _additional_roots = deps_from_parsing_data pd deps.file_system_map filename in
+  let files = List.map (file_of_dep deps.file_system_map []) direct_deps in
+  let inline_ifaces = build_dep_graph_for_files files deps.file_system_map deps.dep_graph deps.parse_results get_parsing_data_from_cache in
+  let filenames, _ = topological_dependences_of deps.file_system_map deps.dep_graph inline_ifaces files false in
+  filenames
+
 (** Collect the dependencies for a list of given files.
     And record the entire dependence graph in the memoized state above **)
 (*
@@ -1478,61 +1552,19 @@ let collect (all_cmd_line_files: list file_name)
           raise_error0 Errors.Fatal_ModuleOrFileNotFound
             (Format.fmt1 "File %s could not be found" fn)
         | Some fn -> fn) in
-  (* The dependency graph; keys are lowercased module names, values = list of
-   * lowercased module names this file depends on. *)
+  // The dependency graph; keys are lowercased module names, values = list of
+  // lowercased module names this file depends on.
   let dep_graph : dependence_graph = deps_empty () in
-
-  (* A map from lowercase module names (e.g. [a.b.c]) to the corresponding
-   * filenames (e.g. [/where/to/find/A.B.C.fst]). Consider this map
-   * immutable from there on. *)
-  let file_system_map = build_map all_cmd_line_files in
-
-  let interfaces_needing_inlining = mk_ref [] in
-  let add_interface_for_inlining l =
-    let l = lowercase_module_name l in
-    interfaces_needing_inlining := l :: !interfaces_needing_inlining
-  in
-
+  // Cached parsing results for each file
   let parse_results = SMap.create 40 in
-
-  (* discover: Do a graph traversal starting from file_name
-   *           filling in dep_graph with the dependences *)
-  let rec discover_one (file_name:file_name) =
-    if deps_try_find dep_graph file_name = None then
-    begin
-      let parsing_data, (deps, mo_roots, needs_interface_inlining) =
-        match SMap.try_find !collect_one_cache file_name with
-        | Some cached -> empty_parsing_data, cached
-        | None ->
-          let parsing_data, deps, needs_interface_inlining, additional_roots = collect_one file_system_map file_name get_parsing_data_from_cache in
-          parsing_data, (deps, additional_roots, needs_interface_inlining)
-      in
-      debug_print (fun _ -> 
-        Format.print3 "collect_one (%s) : deps=%s; mo_roots=%s\n"
-          file_name (show deps) (show mo_roots)
-      );
-      if needs_interface_inlining
-      then add_interface_for_inlining file_name;
-      SMap.add parse_results file_name parsing_data;
-      let deps =
-          let module_name = lowercase_module_name file_name in
-          if is_implementation file_name
-          && has_interface file_system_map module_name
-          then deps @ [UseInterface module_name]
-          else deps
-      in
-      let dep_node : dep_node = {
-        edges = List.unique deps;
-        color = White;
-      } in
-      deps_add_dep dep_graph file_name dep_node;
-      List.iter
-            discover_one
-            (List.map (file_of_dep file_system_map all_cmd_line_files)
-                      (deps @ mo_roots))
-    end
+  // A map from lowercase module names (e.g. [a.b.c]) to the corresponding
+  // filenames (e.g. [/where/to/find/A.B.C.fst]). Consider this map
+  // immutable from there on.
+  let file_system_map = build_map all_cmd_line_files in
+  let inlining_ifaces =
+    build_dep_graph_for_files all_cmd_line_files file_system_map dep_graph parse_results get_parsing_data_from_cache
   in
-  profile (fun () -> List.iter discover_one all_cmd_line_files) "FStarC.Parser.Dep.discover";
+
   debug_print (fun () -> print_graph stdout "stdout" dep_graph file_system_map all_cmd_line_files);
 
   (* At this point, dep_graph has all the (immediate) dependency graph of all the files. *)
@@ -1648,7 +1680,6 @@ let collect (all_cmd_line_files: list file_name)
     let m = lowercase_module_name f in
     Options.add_verify_module m);
 
-  let inlining_ifaces = !interfaces_needing_inlining in
   let all_files, _ =
     profile
       (fun () ->
