src/parser/FStarC.Parser.Dep.fsti
@@ -45,6 +45,9 @@ val interface_of : deps -> module_name:string -> option string  //return value i
 val implementation_of : deps -> module_name:string -> option string  //return value is the file name
 val cache_file_name: (string -> string)
 val parsing_data_of: deps -> string -> parsing_data
+val collect_deps_of_decl (deps:deps) (filename:string) (ds:list FStarC.Parser.AST.decl)
+                          (get_parsing_data_from_cache:string -> option parsing_data)
+: list string //filenames
 val collect: list string -> (string -> option parsing_data) -> list string & deps
 val deps_of : deps -> string -> list string
 val deps_of_modul : deps -> module_name -> list module_name  // list of modules that this module depends on
